case_study/RiscvPmp/Values.v
@@ -50,6 +50,7 @@ Module RiscvPmpValueKit <: ValueKit.
   Notation ty_regidx  := (ty_enum regidx).
   Notation ty_rop     := (ty_enum rop).
   Notation ty_uop     := (ty_enum uop).
+  Notation ty_bop     := (ty_enum bop).
   Notation ty_retired := (ty_enum retired).
 
   (** Unions **)
@@ -59,6 +60,7 @@ Module RiscvPmpValueKit <: ValueKit.
                match K with
                | KRTYPE      => ty_tuple [ty_regidx, ty_regidx, ty_regidx, ty_rop]
                | KUTYPE      => ty_tuple [ty_int, ty_regidx, ty_uop]
+               | KBTYPE      => ty_tuple [ty_int, ty_regidx, ty_regidx, ty_bop]
                | KRISCV_JAL  => ty_tuple [ty_int, ty_regidx]
                | KRISCV_JALR => ty_tuple [ty_int, ty_regidx, ty_regidx]
                end
@@ -70,6 +72,7 @@ Module RiscvPmpValueKit <: ValueKit.
                match Kv with
                | RTYPE rs2 rs1 rd op   => existT KRTYPE (tt , rs2 , rs1 , rd , op)
                | UTYPE imm rd op       => existT KUTYPE (tt , imm , rd , op)
+               | BTYPE imm rs2 rs1 op  => existT KBTYPE (tt , imm , rs2 , rs1 , op)
                | RISCV_JAL imm rd      => existT KRISCV_JAL (tt , imm , rd)
                | RISCV_JALR imm rs1 rd => existT KRISCV_JALR (tt , imm , rs1 , rd)
                end
@@ -79,10 +82,11 @@ Module RiscvPmpValueKit <: ValueKit.
     match U with
     | ast => fun Kv =>
                match Kv with
-               | existT KRTYPE (tt , rs2 , rs1 , rd , op) => RTYPE rs2 rs1 rd op
-               | existT KUTYPE (tt , imm , rd , op)       => UTYPE imm rd op
-               | existT KRISCV_JAL (tt , imm , rd)        => RISCV_JAL imm rd
-               | existT KRISCV_JALR (tt , imm , rs1 , rd) => RISCV_JALR imm rs1 rd
+               | existT KRTYPE (tt , rs2 , rs1 , rd , op)  => RTYPE rs2 rs1 rd op
+               | existT KUTYPE (tt , imm , rd , op)        => UTYPE imm rd op
+               | existT KBTYPE (tt , imm , rs2 , rs1 , op) => BTYPE imm rs2 rs1 op
+               | existT KRISCV_JAL (tt , imm , rd)         => RISCV_JAL imm rd
+               | existT KRISCV_JALR (tt , imm , rs1 , rd)  => RISCV_JALR imm rs1 rd
                end
     end.
 
